RSPDL0 Restriction Semantics

PdlParallelStoring/Completeness.lean
@@ -1,36 +1,75 @@
-import Mathlib.Logic.Basic
-import Mathlib.Data.Set.Insert
+import Mathlib.Data.Finset.Basic
 
 import PdlParallelStoring.AxiomaticSystem
 import PdlParallelStoring.Properties
 
+-- Predicates for formulae and programs in the RSPDL₀ fragment.
+-- In this fragment, we do not allow the use of the operators of:
+--   - test (?)
+--   - iteration (★)
+--   - parallel composition (‖).
+
+inductive RSPDL0Program : π → Prop where
+  | atomic α : RSPDL0Program (π.atomic α)
+  | comp α β : RSPDL0Program α → RSPDL0Program β → RSPDL0Program (α ; β)
+  | choice α β : RSPDL0Program α → RSPDL0Program β → RSPDL0Program (α ∪ β)
+  | s₁ : RSPDL0Program π.s₁
+  | s₂ : RSPDL0Program π.s₂
+  | r₁ : RSPDL0Program π.r₁
+  | r₂ : RSPDL0Program π.r₂
+
+inductive RSPDL0Formula : Φ → Prop where
+  | false : RSPDL0Formula ⊥'
+  | atomic φ : RSPDL0Formula (Φ.atomic φ)
+  | neg φ : RSPDL0Formula φ → RSPDL0Formula (¬ φ)
+  | conj φ₁ φ₂ : RSPDL0Formula φ₁ → RSPDL0Formula φ₂ → RSPDL0Formula (φ₁ ∧ φ₂)
+  | diamond π φ : RSPDL0Program π → RSPDL0Formula φ → RSPDL0Formula (⟨π⟩ φ)
+
+def listToConjunction : List Φ → Φ
+  | [] => ⊤'
+  | [φ] => φ
+  | φ :: φs => φ ∧ listToConjunction φs
+
+noncomputable def finsetToConjunction (φs : Finset Φ) : Φ :=
+  listToConjunction φs.toList
+
 def IsConsistent (s : Set Φ) : Prop :=
-  ¬ ∃ (φs : List Φ), (∀ φ ∈ φs, φ ∈ s) ∧ (⊢ ((φs.foldr (· ∧ ·) ⊤') → ⊥'))
+  (∀ φ ∈ s, RSPDL0Formula φ) ∧
+  ¬ ∃ (φs : Finset Φ), (∀ φ ∈ φs, φ ∈ s) ∧ (⊢ (finsetToConjunction φs → ⊥'))
 
 def IsMaximal (s : Set Φ) : Prop :=
-  IsConsistent s ∧ ∀ {φ : Φ}, (φ ∉ s) → ¬ IsConsistent (s ∪ {φ})
+  IsConsistent s ∧
+  ∀ {φ : Φ}, RSPDL0Formula φ → (φ ∉ s) → ¬ IsConsistent (s ∪ {φ})
 
 def MaximalConsistentSet : Type :=
   {s : Set Φ // IsMaximal s}
 
-def CanonicalFrame : Frame where
+def canonicalRelation (α : π) (Γ Δ : MaximalConsistentSet) : Prop :=
+  ∀ φ, (([α] φ) ∈ Γ.val) → φ ∈ Δ.val
+
+def canonicalFrame : Frame where
   W := MaximalConsistentSet
-  R := sorry
+  R := canonicalRelation
   nonempty := sorry
 
-def CanonicalModel : Model where
-  F := CanonicalFrame
-  V := sorry
+def canonicalValuation (ψ : Ψ) (Γ : MaximalConsistentSet) : Prop :=
+  Φ.atomic ψ ∈ Γ.val
 
-instance canonical_proper : Proper CanonicalFrame := by
+def canonicalModel : Model where
+  F := canonicalFrame
+  V := canonicalValuation
+
+instance canonicalProper : Proper canonicalFrame := by
   sorry
 
-instance canonical_standard : Standard CanonicalModel := by
+instance canonicalStandard : Standard canonicalModel := by
   sorry
 
-instance : ProperStandard CanonicalModel where
-  toStandard := canonical_standard
-  toProper := canonical_proper
+instance : ProperStandard canonicalModel where
+  toStandard := canonicalStandard
+  toProper := canonicalProper
 
-theorem completeness : ∀ {φ : Φ}, (¬ ⊢ φ) → ∃ (M : Model) (_ : ProperStandard M), ¬ (M ⊨ φ) := by
+theorem completeness :
+    ∀ {φ : Φ}, RSPDL0Formula φ → (¬ ⊢ φ) →
+    ∃ (M : Model) (_ : ProperStandard M), ¬ (M ⊨ φ) := by
   sorry
